wip

LeanSubst/Basic.lean
@@ -1,3 +1,4 @@
+module
 
 namespace LeanSubst
 
@@ -5,29 +6,29 @@ universe u u1 u2 u3
 variable {S : Type u1} {T : Type u2} {U : Type u3}
 variable {V : List (Type u2)}
 
-class AltCons (S : outParam $ Type u1) (T : Type u2) where
+public class AltCons (S : outParam $ Type u1) (T : Type u2) where
   altCons : S -> T -> T
 
 infixr:67 (name := «_.:_») " .: " => AltCons.altCons
 
 @[reducible]
-def Subst.typeof {T : Type u2} (_ : T) : Type u2 := T
+public def Subst.typeof {T : Type u2} (_ : T) : Type u2 := T
 
-structure Ren (T : Type u2) : Type u2 where
+public structure Ren (T : Type u2) : Type u2 where
   act : Nat -> Nat
 
-inductive RenVec : List (Type u2) -> Type (u2 + 1)
+public inductive RenVec : List (Type u2) -> Type (u2 + 1)
 | nil : RenVec []
 | cons {T V : _} : Ren T -> RenVec V -> RenVec (T::V)
 
 infixr:67 (name := RenVec.cons_notation) " .: " => RenVec.cons
 
-class RenSuffix (S : Type u1) (V : List (Type u2)) where
+public class RenSuffix (S : Type u1) (V : List (Type u2)) where
 
-class RenMap (S : Type u1) (V : List (Type u2)) where
+public class RenMap (S : Type u1) (V : List (Type u2)) where
   rmap : RenVec V -> S -> S
 
-class inductive RenMapAll : List (Type u2) -> Sort _ where
+public class inductive RenMapAll : List (Type u2) -> Sort _ where
 | nil : RenMapAll []
 | cons {V Vs} [RenMap V (V::Vs)] : RenMapAll Vs -> RenMapAll (V::Vs)
 
@@ -60,11 +61,11 @@ macro_rules
   expand_renvec_lit elems.size (<- `(RenVec.nil))
 
 @[app_unexpander RenVec.nil]
-meta def RenVec.unexpand_nil : Lean.PrettyPrinter.Unexpander
+public meta def RenVec.unexpand_nil : Lean.PrettyPrinter.Unexpander
 | `($(_)) => `(·⟨⟩)
 
 @[app_unexpander RenVec.cons]
-meta def RenVec.unexpand_cons : Lean.PrettyPrinter.Unexpander
+public meta def RenVec.unexpand_cons : Lean.PrettyPrinter.Unexpander
 | `($(_) $x $tail) =>
   match tail with
   | `(·⟨⟩)      => `(·⟨$x⟩)
@@ -73,43 +74,42 @@ meta def RenVec.unexpand_cons : Lean.PrettyPrinter.Unexpander
 | _ => throw ()
 
 @[app_unexpander rmap]
-def unexpand_rmap : Lean.PrettyPrinter.Unexpander
+public meta def unexpand_rmap : Lean.PrettyPrinter.Unexpander
 | `($_ ($r1, RenVec.nil) $t) => `($t⟨$r1⟩)
 | `($_ ($r1, $r2, RenVec.nil) $t) => `($t⟨$r1, $r2⟩)
 | `($_ ($r1, $r2, $r3, RenVec.nil) $t) => `($t⟨$r1, $r2, $r3⟩)
 | `($_ $r $t) => `($t⟨$r,⟩)
 | _ => throw ()
 
-inductive Action (T : Type u2) where
+public inductive Action (T : Type u2) where
 | re : Nat -> Action T
 | su : T -> Action T
-deriving Repr
 
 export Action (re su)
 
-structure Subst (T : Type u2) where
+public structure Subst (T : Type u2) where
   inner : Nat -> Action T
 
-inductive SubstVec : List (Type u2) -> Type (u2 + 1)
+public inductive SubstVec : List (Type u2) -> Type (u2 + 1)
 | nil : SubstVec []
 | cons {T V : _} : Subst T -> SubstVec V -> SubstVec (T::V)
 
 infixr:67 (name := SubstVec.cons_notation) " .: " => SubstVec.cons
 
-class SubstAction (T : Type u1) (A : Type u2) (U : outParam (Type u3)) where
+public class SubstAction (T : Type u1) (A : Type u2) (U : outParam (Type u3)) where
   act (σ : Subst T) : A -> U
 
-def Subst.act [SubstAction S T U] (σ : Subst S) : T -> U := SubstAction.act σ
+public def Subst.act [SubstAction S T U] (σ : Subst S) : T -> U := SubstAction.act σ
 
-instance : SubstAction T Nat (Action T) where
+public instance : SubstAction T Nat (Action T) where
   act := Subst.inner
 
-class SubstSuffix (S : Type u1) (V : List (Type u2)) where
+public class SubstSuffix (S : Type u1) (V : List (Type u2)) where
 
-class SubstMap (S : Type u1) (V : List (Type u2)) where
+public class SubstMap (S : Type u1) (V : List (Type u2)) where
   smap : SubstVec V -> S -> S
 
-class inductive SubstMapAll : List (Type u2) -> Sort _ where
+public class inductive SubstMapAll : List (Type u2) -> Sort _ where
 | nil : SubstMapAll []
 | cons {V Vs} [SubstMap V (V::Vs)] : SubstMapAll Vs -> SubstMapAll (V::Vs)
 
@@ -142,11 +142,11 @@ macro_rules
   expand_substvec_lit elems.size (<- `(SubstVec.nil))
 
 @[app_unexpander SubstVec.nil]
-meta def SubstVec.unexpand_nil : Lean.PrettyPrinter.Unexpander
+public meta def SubstVec.unexpand_nil : Lean.PrettyPrinter.Unexpander
 | `($(_)) => `(·[])
 
 @[app_unexpander SubstVec.cons]
-meta def SubstVec.unexpand_cons : Lean.PrettyPrinter.Unexpander
+public meta def SubstVec.unexpand_cons : Lean.PrettyPrinter.Unexpander
 | `($(_) $x $tail) =>
   match tail with
   | `(·[])      => `(·[$x])
@@ -155,7 +155,7 @@ meta def SubstVec.unexpand_cons : Lean.PrettyPrinter.Unexpander
 | _ => throw ()
 
 @[app_unexpander smap]
-def unexpand_smap : Lean.PrettyPrinter.Unexpander
+public meta def unexpand_smap : Lean.PrettyPrinter.Unexpander
 | `($_ ($σ1, SubstVec.nil) $t) => `($t[$σ1])
 | `($_ ($σ1, $σ2, SubstVec.nil) $t) => `($t[$σ1, $σ2])
 | `($_ ($σ1, $σ2, $σ3, SubstVec.nil) $t) => `($t[$σ1, $σ2, $σ3])
@@ -163,341 +163,341 @@ def unexpand_smap : Lean.PrettyPrinter.Unexpander
 | _ => throw ()
 
 @[reducible, simp]
-instance [i : RenMapAll (T::V)] : RenMap T (T::V) where
+public instance [i : RenMapAll (T::V)] : RenMap T (T::V) where
   rmap :=
     match i with
     | @RenMapAll.cons _ _ i _ => i.rmap
 
 set_option synthInstance.checkSynthOrder false in
 @[reducible, simp]
-instance [i : RenMapAll (T::V)] : RenMapAll V :=
+public instance [i : RenMapAll (T::V)] : RenMapAll V :=
   match i with
   | @RenMapAll.cons _ _ _ i => i
 
 @[reducible, simp]
-instance [i : SubstMapAll (T::V)] : SubstMap T (T::V) where
+public instance [i : SubstMapAll (T::V)] : SubstMap T (T::V) where
   smap :=
     match i with
     | @SubstMapAll.cons _ _ i _ => i.smap
 
 set_option synthInstance.checkSynthOrder false in
 @[reducible, simp]
-instance [i : SubstMapAll (T::V)] : SubstMapAll V :=
+public instance [i : SubstMapAll (T::V)] : SubstMapAll V :=
   match i with
   | @SubstMapAll.cons _ _ _ i => i
 
-def RenVec.head : RenVec (T::V) -> Ren T
+public def RenVec.head : RenVec (T::V) -> Ren T
 | cons r _ => r
 
-def RenVec.tail : RenVec (T::V) -> RenVec V
+public def RenVec.tail : RenVec (T::V) -> RenVec V
 | cons _ r => r
 
 @[simp]
-theorem RenVec.head_cons {r : Ren T} {rs : RenVec V} : (r .: rs).head = r := by simp [head]
+public theorem RenVec.head_cons {r : Ren T} {rs : RenVec V} : (r .: rs).head = r := by simp [head]
 
 @[simp]
-theorem RenVec.tail_cons {r : Ren T} {rs : RenVec V} : (r .: rs).tail = rs := by simp [tail]
+public theorem RenVec.tail_cons {r : Ren T} {rs : RenVec V} : (r .: rs).tail = rs := by simp [tail]
 
-def SubstVec.head : SubstVec (T::V) -> Subst T
+public def SubstVec.head : SubstVec (T::V) -> Subst T
 | cons σ _ => σ
 
-def SubstVec.tail : SubstVec (T::V) -> SubstVec V
+public def SubstVec.tail : SubstVec (T::V) -> SubstVec V
 | cons _ σ => σ
 
 @[simp]
-theorem SubstVec.head_cons {σ : Subst T} {σs : SubstVec V} : (σ .: σs).head = σ := by simp [head]
+public theorem SubstVec.head_cons {σ : Subst T} {σs : SubstVec V} : (σ .: σs).head = σ := by simp [head]
 
 @[simp]
-theorem SubstVec.tail_cons {σ : Subst T} {σs : SubstVec V} : (σ .: σs).tail = σs := by simp [tail]
+public theorem SubstVec.tail_cons {σ : Subst T} {σs : SubstVec V} : (σ .: σs).tail = σs := by simp [tail]
 
 @[simp]
-theorem Subst.act_inner {f : Nat -> Action T} {x} : Subst.act { inner := f } x = f x := by
+public theorem Subst.act_inner {f : Nat -> Action T} {x} : Subst.act { inner := f } x = f x := by
   simp [act, SubstAction.act]
 
 @[simp]
-def Action.rmap1 [RenMap T (T::V)] (r : RenVec (T::V)) : Action T -> Action T
+public def Action.rmap1 [RenMap T (T::V)] (r : RenVec (T::V)) : Action T -> Action T
 | re x => re $ r.head.act x
 | su t => su t⟨r,⟩
 
-instance [RenMap T (T::V)] : RenMap (Action T) (T::V) where
+public instance [RenMap T (T::V)] : RenMap (Action T) (T::V) where
   rmap v := Action.rmap1 v
 
 @[simp]
-theorem Action.rmap1_re [RenMap T (T::V)] {r : RenVec (T::V)} {x : Nat}
+public theorem Action.rmap1_re [RenMap T (T::V)] {r : RenVec (T::V)} {x : Nat}
   : (@re T x)⟨r,⟩ = re (r.head.act x)
 := by simp [RenMap.rmap]
 
 @[simp]
-theorem Action.rmap1_su [RenMap T (T::V)] {r : RenVec (T::V)} {t : T} : (su t)⟨r,⟩ = su t⟨r,⟩ := by
+public theorem Action.rmap1_su [RenMap T (T::V)] {r : RenVec (T::V)} {t : T} : (su t)⟨r,⟩ = su t⟨r,⟩ := by
   simp [RenMap.rmap]
 
 @[simp]
-def Action.rmap0 [RenMap S V] (r : RenVec V) : Action S -> Action S
+public def Action.rmap0 [RenMap S V] (r : RenVec V) : Action S -> Action S
 | re x => re x
 | su t => su t⟨r,⟩
 
-instance [RenMap S V] [RenSuffix S V] : RenMap (Action S) V where
+public instance [RenMap S V] [RenSuffix S V] : RenMap (Action S) V where
   rmap := Action.rmap0
 
 @[simp]
-theorem Action.rmap0_re [RenMap S V] [RenSuffix S V] {r : RenVec V} {x : Nat}
+public theorem Action.rmap0_re [RenMap S V] [RenSuffix S V] {r : RenVec V} {x : Nat}
   : (@re S x)⟨r,⟩ = re x
 := by simp [RenMap.rmap]
 
 @[simp]
-theorem Action.rmap0_su [RenMap S V] [RenSuffix S V] {r : RenVec V} {t : S}
+public theorem Action.rmap0_su [RenMap S V] [RenSuffix S V] {r : RenVec V} {t : S}
   : (su t)⟨r,⟩ = su t⟨r,⟩
 := by simp [RenMap.rmap]
 
 @[simp]
-def Action.smap1 [SubstMap T (T::V)] (σ : SubstVec (T::V)) : Action T -> Action T
+public def Action.smap1 [SubstMap T (T::V)] (σ : SubstVec (T::V)) : Action T -> Action T
 | re x => σ.head.act x
 | su t => su t[σ,]
 
-instance [SubstMap T (T::V)] : SubstMap (Action T) (T::V) where
+public instance [SubstMap T (T::V)] : SubstMap (Action T) (T::V) where
   smap v := Action.smap1 v
 
 @[simp]
-theorem Action.smap1_re [SubstMap T (T::V)] {σ : SubstVec (T::V)} {x : Nat}
+public theorem Action.smap1_re [SubstMap T (T::V)] {σ : SubstVec (T::V)} {x : Nat}
   : (@re T x)[σ,] = σ.head.act x
 := by simp [SubstMap.smap, Subst.act, SubstAction.act]
 
 @[simp]
-theorem Action.smap1_su [SubstMap T (T::V)] {σ : SubstVec (T::V)} {t : T}
+public theorem Action.smap1_su [SubstMap T (T::V)] {σ : SubstVec (T::V)} {t : T}
   : (su t)[σ,] = su t[σ,]
 := by simp [SubstMap.smap]
 
 @[simp]
-def Action.smap0 [SubstMap S V] (σ : SubstVec V) : Action S -> Action S
+public def Action.smap0 [SubstMap S V] (σ : SubstVec V) : Action S -> Action S
 | re x => re x
 | su t => su t[σ,]
 
-instance [SubstMap S V] [SubstSuffix S V] : SubstMap (Action S) V where
+public instance [SubstMap S V] [SubstSuffix S V] : SubstMap (Action S) V where
   smap := Action.smap0
 
 @[simp]
-theorem Action.smap0_re [SubstMap S V] [SubstSuffix S V] {σ : SubstVec V} {x : Nat}
+public theorem Action.smap0_re [SubstMap S V] [SubstSuffix S V] {σ : SubstVec V} {x : Nat}
   : (@re S x)[σ,] = re x
 := by simp [SubstMap.smap]
 
 @[simp]
-theorem Action.smap0_su [SubstMap S V] [SubstSuffix S V] {σ : SubstVec V} {t : S}
+public theorem Action.smap0_su [SubstMap S V] [SubstSuffix S V] {σ : SubstVec V} {t : S}
   : (su t)[σ,] = su t[σ,]
 := by simp [SubstMap.smap]
 
-def Ren.id T : Ren T := ⟨λ x => x⟩
-notation "r+0" => Ren.id _
+public def Ren.id T : Ren T := ⟨λ x => x⟩
+notation "𝐫0" => Ren.id _
 notation "𝐫0(" T ")" => Ren.id T
 
-@[reducible, simp]
-def RenVec.id : (V : List (Type u2)) -> RenVec V
+@[expose, reducible, simp]
+public def RenVec.id : (V : List (Type u2)) -> RenVec V
 | [] => nil
 | .cons x xs => .id x .: id xs
 
-def Subst.id T : Subst T := ⟨λ x => re x⟩
+public def Subst.id T : Subst T := ⟨λ x => re x⟩
 notation "𝐬0" => Subst.id _
 notation "𝐬0(" T ")" => Subst.id T
 
-@[reducible, simp]
-def SubstVec.id : (V : List (Type u2)) -> SubstVec V
+@[expose, reducible, simp]
+public def SubstVec.id : (V : List (Type u2)) -> SubstVec V
 | [] => nil
 | .cons x xs => .id x .: id xs
 
-def Ren.add T (k : Nat) : Ren T := ⟨(· + k)⟩
+public def Ren.add T (k : Nat) : Ren T := ⟨(· + k)⟩
 
-def Subst.add T (k : Nat) : Subst T := ⟨λ x => re $ x + k⟩
+public def Subst.add T (k : Nat) : Subst T := ⟨λ x => re $ x + k⟩
 
-def Ren.sub T (k : Nat) : Ren T := ⟨(· - k)⟩
+public def Ren.sub T (k : Nat) : Ren T := ⟨(· - k)⟩
 
-def Subst.sub T (k : Nat) : Subst T := ⟨λ x => re $ x - k⟩
+public def Subst.sub T (k : Nat) : Subst T := ⟨λ x => re $ x - k⟩
 
-def Ren.cons (a : Nat) (r : Ren T) : Ren T :=
+public def Ren.cons (a : Nat) (r : Ren T) : Ren T :=
   ⟨fun n => match n with
   | 0 => a
   | n + 1 => r.act n⟩
 
-instance : AltCons Nat (Ren T) where
+public instance : AltCons Nat (Ren T) where
   altCons := Ren.cons
 
-def Subst.cons (a : Action T) (σ : Subst T) : Subst T :=
+public def Subst.cons (a : Action T) (σ : Subst T) : Subst T :=
   ⟨fun n => match n with
   | 0 => a
   | n + 1 => σ.act n⟩
 
-instance : AltCons (Action T) (Subst T) where
+public instance : AltCons (Action T) (Subst T) where
   altCons := Subst.cons
 
-def Ren.append : List Nat -> Ren T -> Ren T
+public def Ren.append : List Nat -> Ren T -> Ren T
 | .nil, r => r
 | .cons hd tl, r => hd .: append tl r
 
-instance : HAppend (List Nat) (Ren T) (Ren T) where
+public instance : HAppend (List Nat) (Ren T) (Ren T) where
   hAppend := Ren.append
 
-instance : HAppend (Std.Rco Nat) (Ren T) (Ren T) where
+public instance : HAppend (Std.Rco Nat) (Ren T) (Ren T) where
   hAppend a := Ren.append a.toList
 
-def Subst.append : List (Action T) -> Subst T -> Subst T
+public def Subst.append : List (Action T) -> Subst T -> Subst T
 | .nil, r => r
 | .cons hd tl, r => hd .: append tl r
 
-instance : HAppend (List $ Action T) (Subst T) (Subst T) where
+public instance : HAppend (List $ Action T) (Subst T) (Subst T) where
   hAppend := Subst.append
 
-def Subst.append_ren : List Nat -> Subst T -> Subst T
+public def Subst.append_ren : List Nat -> Subst T -> Subst T
 | .nil, r => r
 | .cons hd tl, r => re hd .: append_ren tl r
 
-instance : HAppend (List Nat) (Subst T) (Subst T) where
+public instance : HAppend (List Nat) (Subst T) (Subst T) where
   hAppend := Subst.append_ren
 
-instance : HAppend (Std.Rco Nat) (Subst T) (Subst T) where
+public instance : HAppend (Std.Rco Nat) (Subst T) (Subst T) where
   hAppend a := Subst.append_ren a.toList
 
-def Ren.compose : Ren T -> Ren T -> Ren T
-| r1, r2 => .mk λ n => r2.act (r1.act n)
+public def Ren.compose : Ren T -> Ren T -> Ren T
+| r1, r2 => ⟨fun n => r2.act (r1.act n)⟩
 
-instance : AndThen (Ren T) where
+public instance : AndThen (Ren T) where
   andThen r f := Ren.compose r (f ())
 
-def RenVec.compose : {V : List (Type u2)} -> RenVec V -> RenVec V -> RenVec V
+public def RenVec.compose : {V : List (Type u2)} -> RenVec V -> RenVec V -> RenVec V
 | _, nil, _ => nil
 | .cons _ _, cons v1 v1s, cons v2 v2s => (v1 >> v2) .: compose v1s v2s
 
-instance : AndThen (RenVec V) where
+public instance : AndThen (RenVec V) where
   andThen r f := RenVec.compose r (f ())
 
-def Subst.compose_ren_left : Ren T -> Subst T -> Subst T
-| r, τ => .mk λ n => τ.act (r.act n)
+public def Subst.compose_ren_left : Ren T -> Subst T -> Subst T
+| r, τ => ⟨fun n => τ.act (r.act n)⟩
 
-instance : HAndThen (Ren T) (Subst T) (Subst T) where
+public instance : HAndThen (Ren T) (Subst T) (Subst T) where
   hAndThen r f := Subst.compose_ren_left r (f ())
 
-def SubstVec.compose_ren_left
+public def SubstVec.compose_ren_left
   : {V : List (Type u2)} -> RenVec V -> SubstVec V -> SubstVec V
 | [],  _, _ => .nil
 | .cons _ _, .cons v1 v1s, cons v2 v2s => (v1 >> v2) .: compose_ren_left v1s v2s
 
-instance : HAndThen (RenVec V) (SubstVec V) (SubstVec V) where
+public instance : HAndThen (RenVec V) (SubstVec V) (SubstVec V) where
   hAndThen r f := SubstVec.compose_ren_left r (f ())
 
-def Subst.compose_ren_right [RenMap T (T::V)] : Subst T -> RenVec (T::V) -> Subst T
-| σ, r => .mk λ n => (σ.act n)⟨r,⟩
+public def Subst.compose_ren_right [RenMap T (T::V)] : Subst T -> RenVec (T::V) -> Subst T
+| σ, r => ⟨fun n => (σ.act n)⟨r,⟩⟩
 
-instance [RenMap T (T::V)] : HAndThen (Subst T) (RenVec (T::V)) (Subst T) where
+public instance [RenMap T (T::V)] : HAndThen (Subst T) (RenVec (T::V)) (Subst T) where
   hAndThen σ f := Subst.compose_ren_right σ (f ())
 
-def SubstVec.compose_ren_right
+public def SubstVec.compose_ren_right
   : {V : List (Type u2)} -> [RenMapAll V] -> SubstVec V -> RenVec V -> SubstVec V
 | [], _, _, _ => .nil
 | .cons _ _, _, cons v1 v1s, v@(.cons _ v2s) => (v1 >> v) .: compose_ren_right v1s v2s
 
-instance [RenMapAll V] : HAndThen (SubstVec V) (RenVec V) (SubstVec V) where
+public instance [RenMapAll V] : HAndThen (SubstVec V) (RenVec V) (SubstVec V) where
   hAndThen σ f := SubstVec.compose_ren_right σ (f ())
 
-def Subst.compose [SubstMap T (T::V)] : Subst T -> SubstVec (T::V) -> Subst T
-| σ, τ => .mk fun n => (σ.act n)[τ,]
+public def Subst.compose [SubstMap T (T::V)] : Subst T -> SubstVec (T::V) -> Subst T
+| σ, τ => ⟨fun n => (σ.act n)[τ,]⟩
 
-instance [SubstMap T (T::V)] : HAndThen (Subst T) (SubstVec (T::V)) (Subst T) where
+public instance [SubstMap T (T::V)] : HAndThen (Subst T) (SubstVec (T::V)) (Subst T) where
   hAndThen σ f := Subst.compose σ (f ())
 
-def SubstVec.compose
+public def SubstVec.compose
   : {V : List (Type u2)} -> [SubstMapAll V] ->
     SubstVec V -> SubstVec V -> SubstVec V
 | [], _, _, _ => .nil
 | .cons _ _, _, cons v1 v1s, v@(cons _ v2s) => (v1 >> v) .: compose v1s v2s
 
-instance [SubstMapAll V] : AndThen (SubstVec V) where
+public instance [SubstMapAll V] : AndThen (SubstVec V) where
   andThen σ f := SubstVec.compose σ (f ())
 
-def Ren.lift (r : Ren T) (k : Nat := 1) : Ren T := (0...k) ++ r >> add T k
+public def Ren.lift (r : Ren T) (k : Nat := 1) : Ren T := (0...k) ++ r >> add T k
 
 @[simp]
-def RenVec.lift : {V : List (Type u2)} -> RenVec V -> List Nat -> RenVec V
+public def RenVec.lift : {V : List (Type u2)} -> RenVec V -> List Nat -> RenVec V
 | [], _, _ => .nil
 | _::_, cons t ts, [] => t .: ts
 | _::_, cons t ts, k::ks => t.lift k .: ts.lift ks
 
-def Subst.lift (V : List (Type u2)) [RenMap T (T::V)] (σ : Subst T) (k : Nat := 1) : Subst T :=
+public def Subst.lift (V : List (Type u2)) [RenMap T (T::V)] (σ : Subst T) (k : Nat := 1) : Subst T :=
   (0...k) ++ σ >> (.add T k .: RenVec.id V)
 
 @[simp]
-def SubstVec.lift : {V : List (Type u2)} -> [RenMapAll V] -> List Nat -> SubstVec V ->  SubstVec V
+public def SubstVec.lift : {V : List (Type u2)} -> [RenMapAll V] -> List Nat -> SubstVec V ->  SubstVec V
 | [], _, _, _ => .nil
 | .cons _ _, _, [], cons t ts => t .: ts
 | .cons _ Vs, _, .cons k ks, cons t ts => t.lift Vs k .: ts.lift ks
 
-def Subst.act_list (σ : Subst T) : (ℓ : List Nat) -> List (Action T)
+public def Subst.act_list (σ : Subst T) : (ℓ : List Nat) -> List (Action T)
 | [] => []
 | .cons x xs => σ.act x :: act_list σ xs
 
-instance : SubstAction T (List Nat) (List (Action T)) where
+public instance : SubstAction T (List Nat) (List (Action T)) where
   act := Subst.act_list
 
-def Ren.to (r : Ren T) : Subst T := ⟨λ x => re (r.act x)⟩
+public def Ren.to (r : Ren T) : Subst T := ⟨λ x => re (r.act x)⟩
 
-def RenVec.to : {V : List (Type u2)} -> RenVec V -> SubstVec V
+public def RenVec.to : {V : List (Type u2)} -> RenVec V -> SubstVec V
 | [], _ => .nil
 | .cons _ _, cons r rs => r.to .: rs.to
 
-class RenMapId (S : Type u1) (V : List (Type u2)) [RenMap S V] where
+public class RenMapId (S : Type u1) (V : List (Type u2)) [RenMap S V] where
   id_law {s : S} : s⟨.id V,⟩ = s
 
 @[simp]
-theorem Ren.id_law [RenMap S V] [RenMapId S V] {s : S} : s⟨.id V,⟩ = s := RenMapId.id_law
+public theorem Ren.id_law [RenMap S V] [RenMapId S V] {s : S} : s⟨.id V,⟩ = s := RenMapId.id_law
 
-class RenMapCompose (S : Type u1) (V : List (Type u2)) [RenMap S V] where
+public class RenMapCompose (S : Type u1) (V : List (Type u2)) [RenMap S V] where
   compose_law {s : S} {r1 r2 : RenVec V} : s⟨r1,⟩⟨r2,⟩ = s⟨r1 >> r2,⟩
 
 @[simp]
-theorem Ren.compose_law [RenMap S V] [RenMapCompose S V] {s : S} {r1 r2 : RenVec V}
+public theorem Ren.compose_law [RenMap S V] [RenMapCompose S V] {s : S} {r1 r2 : RenVec V}
   : s⟨r1,⟩⟨r2,⟩ = s⟨r1 >> r2,⟩
 := RenMapCompose.compose_law
 
-class SubstMapStable (S : Type u1) (V : List $ Type u2) [RenMap S V] [SubstMap S V] where
+public class SubstMapStable (S : Type u1) (V : List $ Type u2) [RenMap S V] [SubstMap S V] where
   stable (r : RenVec V) (σ : SubstVec V) : r.to = σ -> rmap (S := S) r = smap σ
 
 @[grind <-]
-theorem Subst.stable
+public theorem Subst.stable
   [RenMap S V] [SubstMap S V] [SubstMapStable S V]
   {r : RenVec V} {σ : SubstVec V} (h : r.to = σ)
   : rmap (S := S) r = smap σ
 := SubstMapStable.stable _ _ h
 
-class SubstMapId (S : Type u1) (V : List $ Type u2) [SubstMap S V] where
+public class SubstMapId (S : Type u1) (V : List $ Type u2) [SubstMap S V] where
   id_law {s : S} : s[.id V,] = s
 
 @[simp]
-theorem Subst.id_law [SubstMap S V] [SubstMapId S V] {s : S} : s[.id V,] = s :=
+public theorem Subst.id_law [SubstMap S V] [SubstMapId S V] {s : S} : s[.id V,] = s :=
   SubstMapId.id_law
 
-class SubstMapRenComposeLeft (S : Type u1) (V : List $ Type u2) [RenMap S V] [SubstMap S V] where
+public class SubstMapRenComposeLeft (S : Type u1) (V : List $ Type u2) [RenMap S V] [SubstMap S V] where
   compose_left_law {s : S} {r : RenVec V} {τ : SubstVec V} : s⟨r,⟩[τ,] = s[r >> τ,]
 
 @[simp]
-theorem Subst.compose_left_law
+public theorem Subst.compose_left_law
   [RenMap S V] [SubstMap S V] [SubstMapRenComposeLeft S V]
   {s : S} {r : RenVec V} {τ : SubstVec V}
   : s⟨r,⟩[τ,] = s[r >> τ,]
 := SubstMapRenComposeLeft.compose_left_law
 
-class SubstMapRenComposeRight (S : Type u1) (V : List $ Type u2)
+public class SubstMapRenComposeRight (S : Type u1) (V : List $ Type u2)
   [RenMap S V] [RenMapAll V] [SubstMap S V]
 where
   compose_right_law {s : S} {r : RenVec V} {σ : SubstVec V} : s[σ,]⟨r,⟩ = s[σ >> r,]
 
 @[simp]
-theorem Subst.compose_right_law
+public theorem Subst.compose_right_law
   [RenMap S V] [RenMapAll V] [SubstMap S V] [SubstMapRenComposeRight S V]
   {s : S} {σ : SubstVec V} {r : RenVec V}
   : s[σ,]⟨r,⟩ = s[σ >> r,]
 := SubstMapRenComposeRight.compose_right_law
 
-class SubstMapCompose (S : Type u1) (V : List $ Type u2) [SubstMap S V] [SubstMapAll V] where
+public class SubstMapCompose (S : Type u1) (V : List $ Type u2) [SubstMap S V] [SubstMapAll V] where
   compose_law {s : S} {σ τ : SubstVec V} : s[σ,][τ,] = s[σ >> τ,]
 
 @[simp]
-theorem Subst.compose_law
+public theorem Subst.compose_law
   [SubstMap S V] [SubstMapAll V] [SubstMapCompose S V]
   {s : S} {σ τ : SubstVec V}
   : s[σ,][τ,] = s[σ >> τ,]
